CLean/Examples/All.lean
@@ -2,4 +2,5 @@ import CLean.Examples.Common
 import CLean.Examples.Semantic
 import CLean.Examples.Lowering
 import CLean.Examples.Parser
-import CLean.Examples.RealKernels
+import CLean.Examples.Saxpy
+import CLean.Examples.Matmul
